\>{\tiny 1}\'\>\texttt{\textbf{from}}~stack~\texttt{\textbf{import}}~Stack,~\textit{push},~\textit{pop}\\

\>{\tiny 2}\'\>\\

\>{\tiny 3}\'\>\textit{teststack}~=~Stack()\\

\>{\tiny 4}\'\>\textit{push}(?\textit{teststack},~1)\\

\>{\tiny 5}\'\>\textit{push}(?\textit{teststack},~2)\\

\>{\tiny 6}\'\>\textit{v}~=~\textit{pop}(?\textit{teststack})\\

\>{\tiny 7}\'\>\texttt{\textbf{assert}}~\textit{v}~==~2\\

\>{\tiny 8}\'\>\textit{push}(?\textit{teststack},~3)\\

\>{\tiny 9}\'\>\textit{v}~=~\textit{pop}(?\textit{teststack})\\

\>{\tiny 10}\'\>\texttt{\textbf{assert}}~\textit{v}~==~3\\

\>{\tiny 11}\'\>\textit{v}~=~\textit{pop}(?\textit{teststack})\\

\>{\tiny 12}\'\>\texttt{\textbf{assert}}~\textit{v}~==~1